new file:   clojure/for.clj 	modified:   coq/test.v 	new file:   java/Signature.java 	modified:   polyglot/Composite/composite.c 	modified:   polyglot/Composite/composite.t.c 	new file:   sml/sig.sml

clojure/for.clj
@@ -1,0 +1,36 @@
+(def x
+  (for [alpha "abc"
+        beta (range 1 9)
+        gamma '("x23" "x45" "x12")]
+    (str alpha beta gamma)))
+
+; simple trial at emulating nested loops
+(def y
+  (loop [i 0 j 0 k 0 res '()]
+    (if (< i 5)
+      (if (< j 5)
+        (if (< k 5)
+          (recur i j (+ 1 k) (cons [i j k] res))
+          (recur i (+ j 1) 0 res))
+        (recur (+ i 1) 0 0 res))
+      res)))
+
+; semantic equivalent of above 'for' expression
+(def z
+  (loop [alpha "abc" beta (range 1 9) gamma '("x23" "x45" "x12") res '()]
+    (if (not (empty? alpha))
+      (if (not (empty? beta))
+        (if (not (empty? gamma))
+          (recur alpha beta (rest gamma) (cons (str (first alpha) (first beta) (first gamma)) res))
+          (recur alpha (rest beta) '("x23" "x45" "x12") res))
+        (recur (rest alpha) (range 1 9) '("x23" "x45" "x12") res))
+      res)))
+
+
+
+
+
+
+
+(println (sort x))
+(println (sort z))
