java/Signature.java
@@ -1,0 +1,25 @@
+interface MagnitudeObject<T> {
+  int magnitude(T t);
+}
+
+class IntMag implements MagnitudeObject<Integer> {
+  public int magnitude(Integer x){ if (x >= 0) return x; else return -x; }
+}
+
+interface DistanceObject<T> {
+  int distance(T t1, T t2);
+}
+
+class Signature {
+
+  public static void main(String[] args){
+  }
+
+  public static <T> DistanceObject<T> MakeDistanceObject(MagnitudeObject<T> mag){
+    return (x,y) -> {
+      int v = mag.magnitude(x) - mag.magnitude(y);
+      if(v >= 0) return v; else return -v;
+    };
+  }
+
+}
