sml/sig.sml
@@ -1,0 +1,56 @@
+(* interface , typeclass *)
+signature MAG_OBJ =
+  sig
+     type object
+     val mag : object -> int
+  end
+
+(*implementing an interface, declaring a type to 
+* be an instance of a tyepclass *)
+
+structure IntMag : MAG_OBJ = 
+  struct
+    type object = int
+    fun mag(x) = if x >= 0 then x else ~x
+  end
+
+local open IntMag in
+  val y = ~7
+  val z = mag(y)
+end
+
+signature DIST_OBJ =
+  sig
+    type object
+    val dist: object * object -> int
+  end
+
+(* an ML functor is a normal function which takes
+* arguments of type belonging to an interface and returns
+* a value of type belonging to an interface.
+* So a functor is a function between interfaces, or so it seems *)
+
+functor MakeDistObj(structure MAG: MAG_OBJ) =
+  struct
+    type object = MAG.object
+    val dist = fn (x, y) => 
+      let
+        val v = MAG.mag(x) - MAG.mag(y)
+      in
+        if v > 0 then v else ~v 
+      end
+end
+
+
+signature CATEGORY =
+  sig
+    type object
+    type arrow
+    exception uncomposable
+
+    val source: arrow -> object
+    val target: arrow -> object
+    val identity: object -> arrow
+    val composable: arrow * arrow -> bool
+    val compose: arrow * arrow -> arrow
+end
